Bigstar permuting between coordinates

src/examples/matmul-opt/GPU.MatMulOpt.Kernel.fsti
@@ -8,6 +8,7 @@ open Pulse.Lib.BigStar
 open GPU
 open GPU.SizeT
 open GPU.MatMulOpt.Barrier
+open GPU.MatMulOpt.Layout
 module Impure = GPU.MatMulOpt.Impure
 module Pure = GPU.MatMulOpt.Pure
 module SZ = FStar.SizeT
@@ -19,10 +20,18 @@ let blocksize : SZ.t = 32sz
 let tpb : SZ.t = SZ.(blocksize *^ blocksize)
 
 // TODO: un-hardcode
-let rows : SZ.t = 256sz // rows of ga1/r
+let rows : (i: SZ.t { SZ.v i % SZ.v blocksize == 0 }) = 256sz // rows of ga1/r
 // assume val rows : nat
 let shared : SZ.t = 1024sz // columns of ga1, rows of ga2
-let columns : SZ.t = 256sz // columns of ga2/r
+let columns : (i: SZ.t { SZ.v i % SZ.v blocksize == 0 }) = 256sz // columns of ga2/r
+
+let mapping (blocksize: pos) (columns rows: (i: pos { i % blocksize == 0 })) = titi_permutation blocksize blocksize (columns / blocksize) (rows / blocksize)
+let mapping_lemma (blocksize: pos) (columns rows: (i: pos { i % blocksize == 0 })) (tid: nat { tid < rows * columns }):
+  Lemma ((mapping blocksize columns rows).f tid < rows * columns) = ()
+
+let mapping_inv_lemma (blocksize: pos) (columns rows: (i: pos { i % blocksize == 0 })) (tid: nat { tid < rows * columns }):
+  Lemma (tid < blocksize * blocksize * (columns / blocksize) * (rows / blocksize)) = ()
+let mapping_fixed = hide (mapping blocksize columns rows)
 
 let singleton #a (elem: a) : Seq.Base.seq a = Seq.Base.cons elem Seq.Base.empty
 
@@ -31,7 +40,7 @@ let kpre_pair (rows shared columns: nat)
   (ga2: gpu_array U64.t (shared * columns))
   (#s1: erased (Seq.Base.seq U64.t))
   (#s2: erased (Seq.Base.seq U64.t))
-  (size: erased nat { size > 0 })
+  (size: erased pos)
   : slprop
   =
   Impure.gpu_pts_to_matrix rows shared ga1 size s1
@@ -44,12 +53,15 @@ let kpre (shared: nat)
   (r: gpu_array U64.t (rows * columns))
   (#s1: erased (Seq.Base.seq U64.t) )
   (#s2: erased (Seq.Base.seq U64.t))
-  (size: erased nat { reveal size == rows * columns })
-  (tid : nat{ tid < rows * columns})
+  (size: erased pos { reveal size == rows * columns })
+  (idx : nat)
   : slprop
   =
-  kpre_pair rows shared columns ga1 ga2 #s1 #s2 size
-  ** (exists* sr. gpu_pts_to_array_slice r tid (tid+1) sr)
+  kpre_pair rows shared columns ga1 ga2 #s1 #s2 (hide (reveal size))
+  ** (exists* sr. gpu_pts_to_array_slice r idx (idx+1) sr)
+
+let lemma_div_lt (a b: nat) (c: pos): Lemma (requires a < b * c) (ensures 0 <= a / c /\ a / c < b) = ()
+let lemma_mod_lt (a: nat) (c: pos): Lemma (0 <= a % c /\ a % c < c) = ()
 
 let kpost (shared: nat)
   (rows columns: (i: nat { i % SZ.v blocksize == 0 }))
@@ -58,13 +70,14 @@ let kpost (shared: nat)
   (r: gpu_array U64.t (rows * columns))
   (#s1: erased (Seq.Base.seq U64.t) {Seq.Base.length s1 == rows * shared})
   (#s2: erased (Seq.Base.seq U64.t) {Seq.Base.length s2 == shared * columns})
-  (size: erased nat { reveal size == rows * columns })
-  (tid : nat { tid < rows * columns })
+  (size: erased pos { reveal size == rows * columns })
+  (idx : nat { idx < rows * columns })
   : slprop
   =
   Impure.gpu_pts_to_matrix rows shared ga1 size s1
   ** Impure.gpu_pts_to_matrix shared columns ga2 size s2
-  ** gpu_pts_to_array_slice r tid (tid+1) (singleton (Pure.matmul_single rows shared columns s1 s2 (tid / columns) (tid % columns) shared))
+  ** (lemma_div_lt idx rows columns;
+      gpu_pts_to_array_slice r idx (idx+1) (singleton (Pure.matmul_single rows shared columns s1 s2 (idx / columns) (idx % columns) shared)))
   // ** (exists* s. gpu_pts_to_array_slice r tid (tid+1) s)
 
 let shared_pre (nthr : SZ.t { 0 < nthr /\ nthr <= max_threads }) (it: nat) (ar: gpu_array U64.t SZ.(2sz *^ nthr)) (i: nat { 0 <= i /\ i < nthr }): slprop =
@@ -111,6 +124,15 @@ let shared_post (nthr : SZ.t { 0 < nthr /\ nthr <= max_threads }) (ar: gpu_array
   exists* it. shared_pre nthr it ar i
 
 ```pulse
+val fn thread_id_to_idx_2_sz (tid: SZ.t { SZ.v tid < rows * columns })
+  requires emp
+  returns  idx: (i: SZ.t { SZ.v i < rows * columns /\ SZ.v i == (mapping blocksize columns rows).f (SZ.v tid) })
+  ensures  emp
+```
+
+#push-options "--print_implicits --print_bound_var_types"
+
+```pulse
 fn kernel
   // (rows: nat) (shared: nat { shared < pow2 16 }) (columns: nat)
   (ga1 : gpu_array U64.t (rows * shared)) (ga2 : gpu_array U64.t (shared * columns)) (r : gpu_array U64.t (rows * columns))
@@ -124,22 +146,34 @@ fn kernel
   requires gpu
     ** thread_id etid
     ** shared_pre nthr 0 ar (SZ.v (tidx_x etid))
-    ** kpre shared rows columns ga1 ga2 r #s1 #s2 (SZ.v size) (thread_index etid)
+    ** (assert (thread_index etid < rows * columns); mapping_inv_lemma blocksize columns rows (thread_index etid);
+      kpre shared rows columns ga1 ga2 r #s1 #s2 (SZ.v size) (mapping_fixed.f (thread_index etid)))
   ensures  gpu
     ** thread_id etid
     ** shared_post nthr ar (SZ.v (tidx_x etid))
-    ** kpost shared rows columns ga1 ga2 r #s1 #s2 (SZ.v size) (thread_index etid)
+    ** (mapping_lemma blocksize columns rows (thread_index etid); assert (mapping_fixed.f (thread_index etid) < rows * columns);
+      kpost shared rows columns ga1 ga2 r #s1 #s2 (SZ.v size) (mapping_fixed.f (thread_index etid)))
 {
   open FStar.SizeT;
 
+  assert (pure (thread_index etid < rows * columns));
+  mapping_inv_lemma blocksize columns rows (thread_index etid);
+  mapping_lemma blocksize columns rows (thread_index etid);
   let tid : SZ.t = thread_idx_all ();
+  mapping_inv_lemma blocksize columns rows tid;
+  mapping_lemma blocksize columns rows tid;
+  let idx = (mapping_fixed.f (SZ.v tid));
+  let idx_sz = thread_id_to_idx_2_sz tid;
 
-  unfold kpre shared rows columns ga1 ga2 r #s1 #s2 (SZ.v size) (SZ.v tid);
+  unfold kpre shared rows columns ga1 ga2 r #s1 #s2 (SZ.v size) idx;
   unfold kpre_pair rows shared columns ga1 ga2 #s1 #s2 (SZ.v size);
 
   (* r[tid] = TODO *)
-  let trow = SZ.div tid columns;
-  let tcol = SZ.rem tid columns;
+  let trow = SZ.div idx_sz columns;
+  let tcol = SZ.rem idx_sz columns;
+  lemma_div_lt idx_sz rows columns;
+  assume_ (pure (tcol < columns));
+  assert (pure ( idx_sz < rows * columns /\ trow < rows /\ tcol < columns ));
   // assert (pure (0 <= trow /\ trow < rows /\ 0 <= tcol /\ tcol < columns));
 
   let mut i = 0sz;
@@ -171,14 +205,14 @@ fn kernel
   };
 
   let s = !sum;
-  gpu_array_write #U64.t #(rows * columns) #((SZ.v tid)) #((SZ.v tid + 1)) r tid s;
+  gpu_array_write #U64.t #(rows * columns) #idx #(idx + 1) r idx_sz s;
 
-  with #v. assert (gpu_pts_to_array_slice r tid (tid + 1) v);
+  with #v. assert (gpu_pts_to_array_slice r idx (idx + 1) v);
   (**)Seq.Base.lemma_eq_intro v (singleton s);
-  (**)rewrite gpu_pts_to_array_slice r tid (tid + 1) v
-    as gpu_pts_to_array_slice r tid (tid + 1) (singleton s);
+  (**)rewrite gpu_pts_to_array_slice r idx (idx + 1) v
+    as gpu_pts_to_array_slice r idx (idx + 1) (singleton s);
 
-  fold kpost shared rows columns ga1 ga2 r #s1 #s2 (SZ.v size) tid;
+  fold kpost shared rows columns ga1 ga2 r #s1 #s2 (SZ.v size) idx;
   fold shared_post nthr ar (SZ.v (tidx_x etid));
   ()
 }
@@ -225,27 +259,28 @@ ghost fn fold_pre
 ```
 
 
-#push-options "--print_implicits --print_bound_var_types"
+// #push-options "--print_implicits --print_bound_var_types"
 
-```pulse
-ghost fn unfold_post
-  (shared: nat)
-  (rows columns: (i: nat { i % SZ.v blocksize == 0 }))
-  (ga1: gpu_array U64.t (rows * shared))
-  (ga2: gpu_array U64.t (shared * columns))
-  (gr: gpu_array U64.t (rows * columns))
-  (#s1: erased (Seq.Base.seq U64.t) {Seq.Base.length s1 == rows * shared})
-  (#s2: erased (Seq.Base.seq U64.t) {Seq.Base.length s2 == shared * columns})
-  (size: erased nat { reveal size == rows * columns })
-  (tid: nat {  tid < rows * columns })
-  requires kpost shared rows columns ga1 ga2 gr #s1 #s2 size tid
-  ensures  Impure.gpu_pts_to_matrix rows shared ga1 size s1
-        ** Impure.gpu_pts_to_matrix shared columns ga2 size s2
-        ** gpu_pts_to_array_slice gr tid (tid+1) (singleton (Pure.matmul_single rows shared columns s1 s2 (tid / columns) (tid % columns) shared))
-{
-  unfold kpost shared rows columns ga1 ga2 gr #s1 #s2 size tid;
-  ()
-}
-```
+// ```pulse
+// ghost fn unfold_post
+//   (shared: nat)
+//   (rows columns: (i: nat { i % SZ.v blocksize == 0 }))
+//   (ga1: gpu_array U64.t (rows * shared))
+//   (ga2: gpu_array U64.t (shared * columns))
+//   (gr: gpu_array U64.t (rows * columns))
+//   (#s1: erased (Seq.Base.seq U64.t) {Seq.Base.length s1 == rows * shared})
+//   (#s2: erased (Seq.Base.seq U64.t) {Seq.Base.length s2 == shared * columns})
+//   (size: erased nat { reveal size == rows * columns })
+//   (idx: nat { idx < rows * columns })
+//   requires kpost shared rows columns ga1 ga2 gr #s1 #s2 size idx
+//   ensures  Impure.gpu_pts_to_matrix rows shared ga1 size s1
+//         ** Impure.gpu_pts_to_matrix shared columns ga2 size s2
+//         ** (assert (idx < rows * columns /\ idx / columns < rows);
+//             gpu_pts_to_array_slice gr idx (idx+1) (singleton (Pure.matmul_single rows shared columns s1 s2 (idx / columns) (idx % columns) shared)))
+// {
+//   unfold kpost shared rows columns ga1 ga2 gr #s1 #s2 size idx;
+//   ()
+// }
+// ```
 
-#pop-options
+// #pop-options
